examples/store/proofs/server.v
@@ -60,7 +60,7 @@ Lemma wp_server_conn_handler skI skR cs vdb vlock γlock :
 Proof.
 iIntros "#lock #? #ctx".
 iIntros "!> %Φ ((conn & db) & locked) post".
-iPoseProof (RPC.server_connected_keys with "conn") as "#[-> ->]".
+iPoseProof (RPC.server_connected_session with "conn") as "#sess".
 iPoseProof (store_ctx_rpc_ctx with "[//]") as "?".
 wp_lam. wp_pures. wp_list.
 wp_apply wp_server_handle_create; eauto. iIntros "% #?". wp_list.
@@ -72,9 +72,10 @@ wp_apply (RPC.wp_server with "[$conn db]").
   by []. }
 iIntros "(dis & %db & #p_db & vdb & ready)".
 wp_pures.
-rewrite Conn.session_failed_failure.
 wp_apply (release_spec with "[$locked dis vdb ready]") => //.
-iSplit => //. by iFrame.
+iSplit => //. iFrame. iSplit => //.
+iDestruct "ready" as "[fail|?]"; eauto.
+iLeft. by iApply session_compromised'.
 Qed.
 
 Lemma wp_server_find_client ss skI :
